coq/valid_theory.v
@@ -6,7 +6,7 @@ Require Import Lia.
 Require Export lc.tactics.
 Require Import lc.List.
 Require Import lc.Env.
-Require Import lc.SetsAsPredicates.
+Require Import lc.Sets.
 Import SetNotations.
 Local Open Scope set_scope.
 Require Import lc.Monad.
@@ -20,6 +20,22 @@ Require Import lc.model_definitions.
 
 Import EnvNotations.
 Import LCNotations.
+
+Lemma Forall_mem {A}{V : list A}{Pr} : List.Forall Pr V -> Sets.Forall Pr (mem V).
+Proof.
+  induction V; intro h; intros y yIn. 
+  inversion yIn. 
+  inversion h. subst.
+  inversion yIn. subst. auto. eapply IHV; eauto.
+Qed.
+
+(* short proof tactic for goals of the form Sets.Forall success X *)
+Ltac forall_success := 
+  let x:= fresh in 
+  intros x ?; destruct x; try done.
+
+
+#[export] Hint Resolve Forall_mem : core.
 
 Lemma valid_mem_valid {V} : valid_mem V -> valid (mem V).
 Proof.
@@ -39,14 +55,18 @@ Proof. intros. eapply valid_is_nonempty.
 
 (* And do not contain wrong *)
 Lemma valid_not_wrong {X} : valid X -> not (v_wrong ∈ X).
-Proof. intros [x h1]; done. Qed.
+Proof. intros [x h1]. intro h. 
+       specialize (h1 _ h). simpl in h1. done. Qed.
 
 Lemma valid_mem_nonnil {V} : valid_mem V -> V <> nil.
 Proof. intros [h _]; auto. Qed.
 
 Lemma valid_mem_not_wrong {V} : valid_mem V -> not (List.In v_wrong V).
-Proof. intros [h j]; auto. Qed.
-
+Proof. intros [h j]; auto. 
+       rewrite List.Forall_forall in j.
+       intro h1.
+       specialize (j _ h1). simpl in j. done.
+Qed.
 
 (* A finite, inhabited subset of a valid set is valid *)
 Lemma valid_sub_valid_mem {D a} :
@@ -54,8 +74,17 @@ Lemma valid_sub_valid_mem {D a} :
 Proof.
   intros NE [V1 V2] S.
   inversion V1.
+  induction D. try done. 
   split; auto.
+  destruct D.
+  econstructor; eauto. specialize (S a0 ltac:(eauto)). 
+  eapply V2; eauto.
+  econstructor; eauto. specialize (S a0 ltac:(eauto)). 
+  eapply V2; eauto. 
+  eapply IHD. intro h. done. intros y yIn. eapply S.
+  eauto.
 Qed.
+
 
 #[export] Hint Immediate valid_is_nonempty valid_nonempty_mem valid_not_wrong valid_mem_valid valid_mem_nonnil valid_mem_not_wrong valid_sub_valid_mem : core.
 
@@ -67,16 +96,19 @@ Proof.
   intros v1 v2 [[x1 I1] h1] [[x2 I2] h2].
   split. 
   exists x1. eapply Union_introl; eauto.
-  intro h. inversion h; subst; done.
+  intros x xIn. inversion xIn. subst. eapply h1; eauto.
+  eapply h2;eauto.
 Qed.
 
 
 (* valid operators *)
 
+
 Lemma valid_NIL : valid NIL.
 Proof.
   unfold NIL, valid.
-  split. econstructor; eauto. intro h; inversion h.
+  split. econstructor; eauto.
+  forall_success. inversion H0.
 Qed.
 
 Lemma valid_CONS {x y z} : valid x -> valid y -> v_list z ∈ y -> valid (CONS x y).
@@ -84,14 +116,14 @@ Proof.
   intros [[vx h1] nx] [[vl h2] nl] In. unfold CONS.
   split.
   - exists (v_list (vx :: z)). cbv. eauto.
-  - intro h. inversion h.
+  - forall_success. 
 Qed. 
 
 Lemma valid_NAT : forall k, valid (NAT k).
 Proof.
   intros k. unfold NAT, valid. split.
   exists (v_nat k); eauto. cbn. auto.
-  intro h; inversion h.
+  forall_success.
 Qed.
 
 Lemma valid_ADD : valid ADD.
@@ -101,7 +133,7 @@ Proof.
   exists ( (v_list (v_nat 0 :: v_nat 0 :: nil) :: nil) ↦ v_nat 0). 
   cbn.
   exists 0. exists 0. split.  auto. auto.
-  intro h. inversion h.
+  forall_success.
 Qed.
 
 Lemma valid_Λ : forall F, valid (Λ F).
@@ -109,20 +141,20 @@ Proof.
   intros F. 
   split. cbv.
   exists v_fun. auto. 
-  unfold In. done.
+  forall_success.
 Qed.
 
  
 Lemma valid_LIST : forall D, ForallT valid D -> valid (LIST D).
 induction 1. 
 split; auto.
-exists (v_list nil); done. 
+exists (v_list nil); done. forall_success.
 destruct IHX as [[xs nin] h].
 destruct p as [[y niny] hy]. 
 destruct xs; try done.
 split. 
 exists (v_list (y :: l0)). econstructor; eauto.
-eauto.
+forall_success.
 Qed.
 
 (* Valid environments *)
